Semantic alteration? Need to sleep on this

src/Iris/Nola/Syntax.lean
@@ -15,12 +15,48 @@ inductive cif_unsel where
 | /- Basic update -/ cifs_bupd
 | /- Except-0 -/ cifs_except0
 
+set_option pp.universes true
+
 inductive cif (FF : Iris.GFunctors) : Type (u + 1) where
 | /- Universal quantifier -/ cifs_all (A : Type u) (Φ : A -> cif FF)
 | /- Existential quantifier -/ cifs_ex (A : Type u) (Φ : A -> cif FF)
-| /- Binary operator -/ cifs_bin (s : cif_binsel) (P Q : cif FF)
+| /- Binary operator -/ cifs_bin (s : cif_binsel) (P : cif FF) (Q : cif FF)
 | /- Unary operator -/ cifs_un (s : cif_unsel) (P : cif FF)
 | /- Pure proposition -/ cifs_pure (P : Prop)
 | /- Later -/ cifs_later (iP : Iris.IProp FF)
 | /- Invariant -/ cifs_inv (N : Namespace) (fml : cif FF)
 | /- Custom selector -/ cifs_own [Iris.CMRA A] [inG FF A] (a : A)
+
+
+#print cif
+
+open ULift
+
+mutual
+  def lift_cif_to {FF : Iris.GFunctors} : cif.{u} FF → cif.{max u w} FF
+    | cif.cifs_all (A : Type u) Φ =>
+        cif.cifs_all (ULift.{w, u} A) (λ a => lift_cif_to (Φ a.down))
+    | cif.cifs_ex A Φ =>
+        cif.cifs_ex (ULift.{w, u} A) (λ a => lift_cif_to (Φ a.down))
+    | cif.cifs_bin s P Q => cif.cifs_bin s (lift_cif_to P) (lift_cif_to Q)
+    | cif.cifs_un s P    => cif.cifs_un s (lift_cif_to P)
+    | cif.cifs_pure P    => cif.cifs_pure P
+    | cif.cifs_later iP  => cif.cifs_later iP
+    | cif.cifs_inv N P   => cif.cifs_inv N (lift_cif_to P)
+    | @cif.cifs_own _ A _ inst a => @cif.cifs_own _ A _ inst a
+end
+
+def cifs_wandiff {FF} (P Q : cif FF) : cif FF :=
+  cif.cifs_bin cif_binsel.cifs_and
+    (cif.cifs_bin cif_binsel.cifs_wand P Q)
+    (cif.cifs_bin cif_binsel.cifs_wand Q P)
+
+
+def cif_inv {FF} (N : Namespace) (F : cif.{u} FF) : cif.{u + 1} FF :=
+  -- ∃ Q,
+  cif.cifs_ex.{u + 1} (cif.{u} FF) fun Q =>
+    cif.cifs_bin.{u + 1} cif_binsel.cifs_sep
+      -- Q ∗-∗ F
+      ((cifs_wandiff (lift_cif_to.{u, u + 1} Q) (lift_cif_to.{u, u + 1}  F)))
+      -- inv N Q
+      (cif.cifs_inv.{u + 1} N (lift_cif_to.{u, u + 1} Q))
